WIP

pulse/ulib/experimental/Steel.Actions.fst
@@ -141,7 +141,7 @@ let depends_only_on_without_affinity_elim
 
 #push-options "--z3rlimit 100 --max_fuel 1 --initial_fuel 1 --initial_ifuel 0 --max_ifuel 0"
 let pre_action_to_action
-  (fp:hprop) (a: Type) (fp': a -> hprop) (f: pre_action fp a fp')
+  (#fp:hprop) (#a: Type) (#fp': a -> hprop) (f: pre_action fp a fp')
   (action_preserves_frame_disjointness_addr:
     (frame: hprop) ->
     (h0:hheap fp) ->
@@ -390,7 +390,7 @@ let is_m_frame_and_preorder_preserving_intro
 
 #push-options "--z3rlimit 50 --max_ifuel 1 --initial_ifuel 1 --max_fuel 2 --initial_fuel 2"
 let non_alloc_action_to_non_locking_m_action
-  (fp:hprop) (a: Type) (fp': a -> hprop) (f: action fp a fp')
+  (#fp:hprop) (#a: Type) (#fp': a -> hprop) (f: action fp a fp')
     (non_alloc: (h: hheap fp) -> (addr: addr) -> Lemma
     (requires (h addr == None))
     (ensures (let (| _, h'|) = f h in h' addr == None))
@@ -445,8 +445,9 @@ let read_array_addr
   (a:array_ref t)
   (iseq: Ghost.erased (Seq.lseq t (U32.v (length a))))
   (i: U32.t{U32.v i < U32.v (length a)})
-  (p:permission{allows_read p})
-  (m: hheap (pts_to_array a p iseq))
+  (p: permission{allows_read p})
+  (pre: Ghost.erased (Preorder.preorder t))
+  (m: hheap (pts_to_array_with_preorder a p iseq pre))
   : Tot (x:t{x == Seq.index iseq (U32.v i)})
   =
   match m a.array_addr with
@@ -463,12 +464,13 @@ let index_array_pre_action
   (iseq: Ghost.erased (Seq.lseq t (U32.v (length a))))
   (i: U32.t{U32.v i < U32.v (length a)})
   (p:permission{allows_read p})
+  (pre: Ghost.erased (Preorder.preorder t))
   : Tot (pre_action
-    (pts_to_array a p iseq)
+    (pts_to_array_with_preorder a p iseq pre)
     (x:t{x == Seq.index iseq (U32.v i)})
-    (fun _ -> pts_to_array a p iseq))
+    (fun _ -> pts_to_array_with_preorder a p iseq pre))
   = fun h ->
-  let x = read_array_addr a iseq i p h in
+  let x = read_array_addr a iseq i p pre h in
   (| x, h |)
 
 let index_array_action
@@ -477,16 +479,15 @@ let index_array_action
   (iseq: Ghost.erased (Seq.lseq t (U32.v (length a))))
   (i: U32.t{U32.v i < U32.v (length a)})
   (p:permission{allows_read p})
+  (pre: Ghost.erased (Preorder.preorder t))
   : Tot (pre_action
-    (pts_to_array a p iseq)
+    (pts_to_array_with_preorder a p iseq pre)
     (x:t{x == Seq.index iseq (U32.v i)})
-    (fun _ -> pts_to_array a p iseq))
+    (fun _ -> pts_to_array_with_preorder a p iseq pre))
   =
   pre_action_to_action
-    (pts_to_array a p iseq)
-    (x:t{x == Seq.index iseq (U32.v i)})
-    (fun _ -> pts_to_array a p iseq)
-    (index_array_pre_action a iseq i p)
+
+    (index_array_pre_action a iseq i p pre)
     (fun frame h0 h1 addr -> ())
     (fun frame h0 h1 addr -> ())
     (fun frame h0 h1 -> ())
@@ -498,30 +499,25 @@ let index_array
   (p: permission{allows_read p})
   (i:U32.t{U32.v i < U32.v (length a)}) =
   non_alloc_action_to_non_locking_m_action
-    (pts_to_array a p iseq)
-    (x:t{x == Seq.index iseq (U32.v i)})
-    (fun _ -> pts_to_array a p iseq)
-    (index_array_action a iseq i p)
+    (index_array_action a iseq i p (trivial_preorder t))
     (fun h addr -> ())
 
 let update_array_addr
   (#t:_)
   (a: array_ref t)
+  (iseq:  Ghost.erased (Seq.lseq t (U32.v (length a))))
   (i:U32.t{U32.v i < U32.v (length a)})
   (v: t)
   (perm:permission{allows_read perm})
-  (m: heap{match m a.array_addr with
-    | Some (Array t' len seq) ->
-      t' == t /\ U32.v (offset a) + U32.v (length a) <= len
-    | _ -> False
-  })
+  (pre: (Ghost.erased (Preorder.preorder t)){(Ghost.reveal pre) (Seq.index iseq (U32.v i)) v})
+  (m: hheap (pts_to_array_with_preorder a perm iseq pre))
   =
   match m a.array_addr with
   | Some (Array t' len seq) ->
     on _ (fun a' ->
       if a.array_addr = a' then
         let new_seq = Seq.upd seq (U32.v i + U32.v a.array_offset) (Some ({
-          value = v; perm =  perm; preorder = trivial_preorder t
+          value = v; perm =  perm; preorder = pre
         })) in
         Some (Array t len new_seq)
       else
@@ -536,9 +532,10 @@ let upd_array_heap
   (iseq:  Ghost.erased (Seq.lseq t (U32.v (length a))))
   (i:U32.t{U32.v i < U32.v (length a)})
   (v: t)
-  (h: hheap (pts_to_array a full_permission iseq)) : heap =
+  (pre: (Ghost.erased (Preorder.preorder t)){(Ghost.reveal pre) (Seq.index iseq (U32.v i)) v})
+  (h: hheap (pts_to_array_with_preorder a full_permission iseq pre)) : heap =
   let Array _ len v_orig = select_addr h a.array_addr in
-  update_array_addr a i v full_permission h
+  update_array_addr a iseq i v full_permission pre h
 #pop-options
 
 #push-options "--z3rlimit 15 --max_fuel 2 --initial_fuel 2 --initial_ifuel 1 --max_ifuel 1"
@@ -548,21 +545,21 @@ let upd_array_heap_frame_disjointness_preservation
   (iseq: Ghost.erased (Seq.lseq t (U32.v (length a))))
   (i:U32.t{U32.v i < U32.v (length a)})
   (v: t)
+  (pre: (Ghost.erased (Preorder.preorder t)){(Ghost.reveal pre) (Seq.index iseq (U32.v i)) v})
   (h h0 h1:heap)
   (frame:hprop)
   : Lemma
     (requires
       disjoint h0 h1 /\
       h == join h0 h1 /\
-      interp (pts_to_array a full_permission iseq) h0 /\
+      interp (pts_to_array_with_preorder a full_permission iseq pre) h0 /\
       interp frame h1)
     (ensures (
-      let h0' = upd_array_heap a iseq i v h0 in
+      let h0' = upd_array_heap a iseq i v pre h0 in
       disjoint h0' h1))
   =
   ()
 #pop-options
-
 
 let upd_array_pre_action
   (#t:_)
@@ -570,40 +567,44 @@ let upd_array_pre_action
   (iseq:  Ghost.erased (Seq.lseq t (U32.v (length a))))
   (i:U32.t{U32.v i < U32.v (length a)})
   (v: t)
+  (pre: (Ghost.erased (Preorder.preorder t)){(Ghost.reveal pre) (Seq.index iseq (U32.v i)) v})
   : pre_action
-    (pts_to_array a full_permission iseq)
+    (pts_to_array_with_preorder a full_permission iseq pre)
     unit
-    (fun _ -> pts_to_array a full_permission (Seq.upd iseq (U32.v i) v))
+    (fun _ -> pts_to_array_with_preorder a full_permission (Seq.upd iseq (U32.v i) v) pre)
   = fun h ->
-    (| (), upd_array_heap a iseq i v h |)
+    (| (), upd_array_heap a iseq i v pre h |)
 
-#push-options "--z3rlimit 150 --max_fuel 1 --initial_fuel 1 --initial_ifuel 1 --max_ifuel 1"
+#push-options "--z3rlimit 150 --max_fuel 2 --initial_fuel 2 --initial_ifuel 1 --max_ifuel 1"
 let upd_array_action_memory_split_independence
   (#t:_)
   (a:array_ref t)
   (iseq: Ghost.erased (Seq.lseq t (U32.v (length a))))
   (i:U32.t{U32.v i < U32.v (length a)})
   (v: t)
+  (pre: (Ghost.erased (Preorder.preorder t)){(Ghost.reveal pre) (Seq.index iseq (U32.v i)) v})
   (h h0 h1:heap)
   (frame:hprop)
   : Lemma
     (requires
       disjoint h0 h1 /\
       h == join h0 h1 /\
-      interp (pts_to_array a full_permission iseq) h0 /\
+      interp (pts_to_array_with_preorder a full_permission iseq pre) h0 /\
       interp frame h1)
     (ensures (
-      let (| _, h' |) = upd_array_pre_action a iseq i v h in
-      let h0' = upd_array_heap a iseq i v h0 in
-      upd_array_heap_frame_disjointness_preservation a iseq i v h h0 h1 frame;
+      let (| _, h' |) = upd_array_pre_action a iseq i v pre h in
+      let h0' = upd_array_heap a iseq i v pre h0 in
+      upd_array_heap_frame_disjointness_preservation a iseq i v pre h h0 h1 frame;
       h' == (join h0' h1)))
   =
-  let (| _, h' |) = upd_array_pre_action a iseq i v h in
-  let h0' = upd_array_heap a iseq i v h0 in
-  upd_array_heap_frame_disjointness_preservation a iseq i v h h0 h1 frame;
+  let (| _, h' |) = upd_array_pre_action a iseq i v pre h in
+  let h0' = upd_array_heap a iseq i v pre h0 in
+  upd_array_heap_frame_disjointness_preservation a iseq i v pre h h0 h1 frame;
   assert(disjoint h0' h1);
   let aux (addr: addr) : Lemma (
-    h' addr == (join h0' h1) addr
+    upd_array_heap_frame_disjointness_preservation a iseq i v pre h h0 h1 frame;
+    assert(disjoint h0' h1);
+    h' addr == (join h0' (h1 <: (m1:heap{disjoint h0' m1}))) addr
   ) =
     if addr <> a.array_addr then () else
     if not (h1 `contains_addr` addr) then ()
@@ -622,27 +623,25 @@ let upd_array_action
   (iseq: Ghost.erased (Seq.lseq t (U32.v (length a))))
   (i:U32.t{U32.v i < U32.v (length a)})
   (v: t)
+  (pre: (Ghost.erased (Preorder.preorder t)){(Ghost.reveal pre) (Seq.index iseq (U32.v i)) v})
   : Tot (
     action
-      (pts_to_array a full_permission iseq)
+      (pts_to_array_with_preorder a full_permission iseq pre)
       unit
-      (fun _ -> pts_to_array a full_permission (Seq.upd iseq (U32.v i) v))
+      (fun _ -> pts_to_array_with_preorder a full_permission (Seq.upd iseq (U32.v i) v) pre)
     )
   =
   pre_action_to_action
-    (pts_to_array a full_permission iseq)
-    unit
-    (fun _ -> pts_to_array a full_permission (Seq.upd iseq (U32.v i) v))
-    (upd_array_pre_action a iseq i v)
+    (upd_array_pre_action a iseq i v pre)
     (fun frame h0 h1 addr -> (* Disjointness preservation *)
-      upd_array_heap_frame_disjointness_preservation a iseq i v (join h0 h1) h0 h1 frame
+      upd_array_heap_frame_disjointness_preservation a iseq i v pre (join h0 h1) h0 h1 frame
     )
     (fun frame h0 h1 addr -> (* Does not depend on framing *)
-      upd_array_action_memory_split_independence a iseq i v (join h0 h1) h0 h1 frame
+      upd_array_action_memory_split_independence a iseq i v pre (join h0 h1) h0 h1 frame
     )
     (fun frame h0 h1 -> (* Return  *)
-      let (| x0, h |) = upd_array_pre_action a iseq i v h0 in
-      let (| x1, h' |) = upd_array_pre_action a iseq i v (join h0 h1) in
+      let (| x0, h |) = upd_array_pre_action a iseq i v pre h0 in
+      let (| x1, h' |) = upd_array_pre_action a iseq i v pre (join h0 h1) in
       assert (x0 == x1)
     )
 
@@ -658,31 +657,20 @@ let upd_array
     (fun _ -> pts_to_array a full_permission (Seq.upd iseq (U32.v i) v))
   =
   non_alloc_action_to_non_locking_m_action
-    (pts_to_array a full_permission iseq)
-    unit
-    (fun _ -> pts_to_array a full_permission (Seq.upd iseq (U32.v i) v))
-    (upd_array_action a iseq i v)
+    (upd_array_action a iseq i v (trivial_preorder t))
     (fun h addr -> ())
-
-// MST = MST mem locks_preorder
-
-// let (:=) #a r v
-// : action_t (ptr r) (fun _ -> points_to r v) (fun _ -> True)
-//   (fun h0 _ h1 -> True)
-//   let m = MST.get () in
-//   let m1 = upd r v m in
-//   MST.put m1
 
 let singleton_heap
   (#t: _)
   (len:U32.t)
   (init: t)
+  (pre: Ghost.erased (Preorder.preorder t))
   (a: array_ref t{
     U32.v len = U32.v a.array_length /\
     U32.v len = U32.v a.array_max_length /\
     0 = U32.v a.array_offset
   })
-  : hheap (pts_to_array a full_permission (Seq.Base.create (U32.v len) init))
+  : hheap (pts_to_array_with_preorder a full_permission (Seq.Base.create (U32.v len) init) pre)
   =
   let h = on _ (fun a' ->
     if a' <> a.array_addr then None else
@@ -690,22 +678,22 @@ let singleton_heap
       Some ({
         value = init;
         perm = (full_permission <: (perm:permission{allows_read perm}));
-        preorder = trivial_preorder t
+        preorder = pre
       })
     )))
   ) in
   h
-
 
 #push-options "--z3rlimit 50 --max_fuel 2 --initial_fuel 2 --initial_ifuel 1 --max_ifuel 1 --warn_error -271"
 let alloc_array_pre_m_action
   (#t: _)
   (len:U32.t)
   (init: t)
+  (pre: Ghost.erased (Preorder.preorder t))
   : pre_m_action
     emp
     (a:array_ref t{length a = len /\ offset a = 0ul /\ max_length a = len})
-    (fun a -> pts_to_array a full_permission (Seq.Base.create (U32.v len) init))
+    (fun a -> pts_to_array_with_preorder a full_permission (Seq.Base.create (U32.v len) init) pre)
   =  fun m ->
   let a = {
     array_addr = m.ctr;
@@ -713,14 +701,19 @@ let alloc_array_pre_m_action
     array_length = len;
     array_offset = 0ul;
   } in
-  let single_h = singleton_heap len init a in
+  let single_h = singleton_heap len init pre a in
   let new_h = join (heap_of_mem m) single_h in
   assert(forall i. i>= m.ctr + 1 ==> new_h i == None);
   assert(disjoint m.heap single_h);
   assert(interp (lock_store_invariant m.locks) (heap_of_mem m));
-  assert(interp (pts_to_array a full_permission (Seq.Base.create (U32.v len) init)) single_h);
-  assert(interp ((pts_to_array a full_permission (Seq.Base.create (U32.v len) init))
-    `star` (lock_store_invariant m.locks)) new_h);
+  assert(interp (
+    pts_to_array_with_preorder a full_permission (Seq.Base.create (U32.v len) init) pre)
+    single_h
+  );
+  assert(interp (
+    (pts_to_array_with_preorder a full_permission (Seq.Base.create (U32.v len) init) pre)
+    `star` (lock_store_invariant m.locks)) new_h
+  );
   let new_m = { m with heap = new_h; ctr = m.ctr +1 } in
   (| a, new_m |)
 #pop-options
@@ -740,15 +733,17 @@ let ac_reasoning_for_m_frame_preserving'
   assert (interp (p `star` (q `star` r)) (heap_of_mem m));
   affine_star p (q `star` r) (heap_of_mem m)
 
-
 #push-options " --max_fuel 0 --initial_fuel 0 --initial_ifuel 0 --max_ifuel 0"
 let alloc_array_is_m_frame_and_preorder_preserving
   (#t: _)
   (len:U32.t)
   (init: t)
-  : Lemma (is_m_frame_and_preorder_preserving (alloc_array_pre_m_action len init))
+  (pre: Preorder.preorder t)
+  : Lemma (is_m_frame_and_preorder_preserving (
+    alloc_array_pre_m_action len init pre)
+  )
   =
-  is_m_frame_and_preorder_preserving_intro (alloc_array_pre_m_action len init) (fun frame m ->
+  is_m_frame_and_preorder_preserving_intro (alloc_array_pre_m_action len init pre) (fun frame m ->
     let h = heap_of_mem m in
     let a : array_ref t = {
       array_addr = m.ctr;
@@ -757,37 +752,39 @@ let alloc_array_is_m_frame_and_preorder_preserving
       array_offset = 0ul;
     } in
     ac_reasoning_for_m_frame_preserving emp frame (locks_invariant m) m;
-    let (| a, m1 |) = alloc_array_pre_m_action len init m in
+    let (| a, m1 |) = alloc_array_pre_m_action len init pre m in
     assert (m1.ctr = m.ctr + 1);
     assert (m1.locks == m.locks);
     let h1 = heap_of_mem m1 in
-    let single_h = singleton_heap len init a in
+    let single_h = singleton_heap len init pre a in
     assert (h1 == join single_h h);
     intro_pts_to_array_with_preorder
-      a full_permission (Seq.Base.create (U32.v len) init) (trivial_preorder t) single_h;
-    assert (interp (pts_to_array a full_permission (Seq.Base.create (U32.v len) init)) single_h);
+      a full_permission (Seq.Base.create (U32.v len) init) pre single_h;
+    assert (interp (
+      pts_to_array_with_preorder a full_permission (Seq.Base.create (U32.v len) init) pre) single_h
+    );
     ac_reasoning_for_m_frame_preserving' emp frame (locks_invariant m) m;
     assert (interp (frame `star` locks_invariant m) h);
     intro_star
-      (pts_to_array a full_permission (Seq.Base.create (U32.v len) init))
+      (pts_to_array_with_preorder a full_permission (Seq.Base.create (U32.v len) init) pre)
       (frame `star` locks_invariant m)
       single_h
       h;
     assert (interp
-      (pts_to_array a full_permission (Seq.Base.create (U32.v len) init) `star`
-      (frame `star` locks_invariant m)) h1
+      (pts_to_array_with_preorder a full_permission (Seq.Base.create (U32.v len) init) pre
+      `star` (frame `star` locks_invariant m)) h1
     );
     star_associative
-      (pts_to_array a full_permission (Seq.Base.create (U32.v len) init))
+      (pts_to_array_with_preorder a full_permission (Seq.Base.create (U32.v len) init) pre)
       frame
       (locks_invariant m);
     assert (interp
-      (pts_to_array a full_permission (Seq.Base.create (U32.v len) init) `star`
-      frame `star` locks_invariant m) h1
+      (pts_to_array_with_preorder a full_permission (Seq.Base.create (U32.v len) init) pre
+      `star` frame `star` locks_invariant m) h1
     );
     assert(mem_evolves m m1)
   ) (fun frame m f_frame ->
-   let h = heap_of_mem m in
+    let h = heap_of_mem m in
     let a : array_ref t = {
       array_addr = m.ctr;
       array_max_length = len;
@@ -795,11 +792,11 @@ let alloc_array_is_m_frame_and_preorder_preserving
       array_offset = 0ul;
     } in
     ac_reasoning_for_m_frame_preserving emp frame (locks_invariant m) m;
-    let (| a, m1 |) = alloc_array_pre_m_action len init m in
+    let (| a, m1 |) = alloc_array_pre_m_action len init pre m in
     assert (m1.ctr = m.ctr + 1);
     assert (m1.locks == m.locks);
     let h1 = heap_of_mem m1 in
-    let single_h = singleton_heap len init a in
+    let single_h = singleton_heap len init pre a in
     assert (h1 == join single_h h);
     assert(depends_only_on_without_affinity f_frame frame);
     assert (interp ((emp `star` frame) `star` (locks_invariant m)) h);
@@ -819,8 +816,8 @@ let alloc_array
     (a:array_ref t{length a = len /\ offset a = 0ul /\ max_length a = len})
     (fun a -> pts_to_array a full_permission (Seq.Base.create (U32.v len) init))
   =
-  alloc_array_is_m_frame_and_preorder_preserving len init;
-  alloc_array_pre_m_action len init
+  alloc_array_is_m_frame_and_preorder_preserving len init (trivial_preorder t);
+  alloc_array_pre_m_action len init (trivial_preorder t)
 
 let free_array_pre_action
   (#t: _)
@@ -836,9 +833,6 @@ let free_array_action
   (a: array_ref t{freeable a})
   =
   pre_action_to_action
-    (array_perm a full_permission)
-    unit
-    (fun _ -> emp)
     (free_array_pre_action a)
     (fun frame h0 h1 addr -> ())
     (fun frame h0 h1 post -> ())
@@ -853,9 +847,6 @@ let free_array
     (fun _ -> emp)
   =
   non_alloc_action_to_non_locking_m_action
-    (array_perm a full_permission)
-    unit
-    (fun _ -> emp)
     (free_array_action a)
     (fun h addr -> ())
 
@@ -865,15 +856,16 @@ let share_array_pre_action
   (a: array_ref t)
   (iseq: Ghost.erased (Seq.lseq t (U32.v (length a))))
   (perm: permission{allows_read perm})
+  (pre: Ghost.erased (Preorder.preorder t))
   : pre_action
-    (pts_to_array a perm iseq)
+    (pts_to_array_with_preorder a perm iseq pre)
     (a':array_ref t{
       length a' = length a /\ offset a' = offset a /\ max_length a' = max_length a /\
       address a = address a'
     })
     (fun a' -> star
-      (pts_to_array a (half_permission perm) iseq)
-      (pts_to_array a' (half_permission perm) (Ghost.hide (Ghost.reveal iseq)))
+      (pts_to_array_with_preorder a (half_permission perm) iseq pre)
+      (pts_to_array_with_preorder a' (half_permission perm) (Ghost.hide (Ghost.reveal iseq)) pre)
     )
     = fun h ->
       let split_h_1 : heap = on _ (fun addr ->
@@ -928,33 +920,25 @@ let share_array_action
   (a: array_ref t)
   (iseq: Ghost.erased (Seq.lseq t (U32.v (length a))))
   (perm: permission{allows_read perm})
+  (pre: Ghost.erased (Preorder.preorder t))
   : action
-    (pts_to_array a perm iseq)
+    (pts_to_array_with_preorder a perm iseq pre)
     (a':array_ref t{
       length a' = length a /\ offset a' = offset a /\ max_length a' = max_length a /\
       address a = address a'
     })
     (fun a' -> star
-      (pts_to_array a (half_permission perm) iseq)
-      (pts_to_array a' (half_permission perm) (Ghost.hide (Ghost.reveal iseq)))
+      (pts_to_array_with_preorder a (half_permission perm) iseq pre)
+      (pts_to_array_with_preorder a' (half_permission perm) (Ghost.hide (Ghost.reveal iseq)) pre)
     )
   =
   pre_action_to_action
-    (pts_to_array a perm iseq)
-    (a':array_ref t{
-      length a' = length a /\ offset a' = offset a /\ max_length a' = max_length a /\
-      address a = address a'
-    })
-    (fun a' -> star
-      (pts_to_array a (half_permission perm) iseq)
-      (pts_to_array a' (half_permission perm) (Ghost.hide (Ghost.reveal iseq)))
-    )
-    (share_array_pre_action a iseq perm)
+    (share_array_pre_action a iseq perm pre)
     (fun frame h0 h1 addr -> ())
     (fun frame h0 h1 addr -> ())
     (fun frame h0 h1 ->
-      let (|x_alone, h0'|) = share_array_pre_action a iseq perm h0 in
-      let (|x_joint, h'|) = share_array_pre_action a iseq perm (join h0 h1) in
+      let (|x_alone, h0'|) = share_array_pre_action a iseq perm pre h0 in
+      let (|x_joint, h'|) = share_array_pre_action a iseq perm pre (join h0 h1) in
       assert(x_alone == x_joint)
     )
 
@@ -975,17 +959,8 @@ let share_array
     )
     =
     non_alloc_action_to_non_locking_m_action
-       (pts_to_array a perm iseq)
-    (a':array_ref t{
-      length a' = length a /\ offset a' = offset a /\ max_length a' = max_length a /\
-      address a = address a'
-    })
-    (fun a' -> star
-      (pts_to_array a (half_permission perm) iseq)
-      (pts_to_array a' (half_permission perm) (Ghost.hide (Ghost.reveal iseq)))
-    )
-    (share_array_action a iseq perm)
-    (fun h addr -> ())
+      (share_array_action a iseq perm (trivial_preorder t))
+      (fun h addr -> ())
 
 #push-options "--max_fuel 2 --initial_fuel 2 --max_ifuel 1 --initial_ifuel 1 --z3rlimit 40"
 let gather_array_pre_action
@@ -998,13 +973,14 @@ let gather_array_pre_action
   (iseq: Ghost.erased (Seq.lseq t (U32.v (length a))))
   (p: permission{allows_read p})
   (p': permission{allows_read p' /\ summable_permissions p p'})
+  (pre: Ghost.erased (Preorder.preorder t))
   : pre_action
     (star
-      (pts_to_array a p iseq)
-      (pts_to_array a' p' (Ghost.hide (Ghost.reveal iseq)))
+      (pts_to_array_with_preorder a p iseq pre)
+      (pts_to_array_with_preorder a' p' (Ghost.hide (Ghost.reveal iseq)) pre)
     )
     unit
-    (fun _ -> pts_to_array a (sum_permissions p p') iseq)
+    (fun _ -> pts_to_array_with_preorder a (sum_permissions p p') iseq pre)
   = fun h ->
     (| (), h |)
 #pop-options
@@ -1020,22 +996,17 @@ let gather_array_action
   (iseq: Ghost.erased (Seq.lseq t (U32.v (length a))))
   (p: permission{allows_read p})
   (p': permission{allows_read p' /\ summable_permissions p p'})
+  (pre: Ghost.erased (Preorder.preorder t))
   : action
     (star
-      (pts_to_array a p iseq)
-      (pts_to_array a' p' (Ghost.hide (Ghost.reveal iseq)))
+      (pts_to_array_with_preorder a p iseq pre)
+      (pts_to_array_with_preorder a' p' (Ghost.hide (Ghost.reveal iseq)) pre)
     )
     unit
-    (fun _ -> pts_to_array a (sum_permissions p p') iseq)
+    (fun _ -> pts_to_array_with_preorder a (sum_permissions p p') iseq pre)
   =
   pre_action_to_action
-    (star
-      (pts_to_array a p iseq)
-      (pts_to_array a' p' (Ghost.hide (Ghost.reveal iseq)))
-    )
-    unit
-    (fun _ -> pts_to_array a (sum_permissions p p') iseq)
-    (gather_array_pre_action a a' iseq p p')
+    (gather_array_pre_action a a' iseq p p' pre)
     (fun frame h0 h1 addr -> ())
     (fun frame h0 h1 addr -> ())
     (fun frame h0 h1 -> ())
@@ -1060,13 +1031,7 @@ let gather_array
     (fun _ -> pts_to_array a (sum_permissions p p') iseq)
     =
     non_alloc_action_to_non_locking_m_action
-      (star
-        (pts_to_array a p iseq)
-        (pts_to_array a' p' (Ghost.hide (Ghost.reveal iseq)))
-      )
-      unit
-      (fun _ -> pts_to_array a (sum_permissions p p') iseq)
-      (gather_array_action a a' iseq p p')
+      (gather_array_action a a' iseq p p' (trivial_preorder t))
       (fun h addr -> ())
 
 #push-options "--max_fuel 2 --initial_fuel 2 --max_ifuel 1 --initial_ifuel 1 --z3rlimit 150"
@@ -1076,8 +1041,9 @@ let split_array_pre_action
   (iseq: Ghost.erased (Seq.lseq t (U32.v (length a))))
   (p: permission{allows_read p})
   (i:U32.t{U32.v i < U32.v (length a)})
+  (pre: Ghost.erased (Preorder.preorder t))
   : pre_action
-    (pts_to_array a p iseq)
+    (pts_to_array_with_preorder a p iseq pre)
     (as:(array_ref t & array_ref t){(
       length (fst as) = i /\ length (snd as) = U32.sub (length a) i /\
       offset (fst as) = offset a /\ offset (snd as) = U32.add (offset a) i /\
@@ -1085,8 +1051,8 @@ let split_array_pre_action
       address (fst as) = address a /\ address (snd as) = address a
     )})
     (fun (a1, a2) -> star
-      (pts_to_array a1 p (Seq.slice iseq 0 (U32.v i)))
-      (pts_to_array a2 p (Seq.slice iseq (U32.v i) (U32.v (length a))))
+      (pts_to_array_with_preorder a1 p (Seq.slice iseq 0 (U32.v i)) pre)
+      (pts_to_array_with_preorder a2 p (Seq.slice iseq (U32.v i) (U32.v (length a))) pre)
     )
   = fun h ->
   let a1 = { a with
@@ -1147,8 +1113,9 @@ let split_array_action
   (iseq: Ghost.erased (Seq.lseq t (U32.v (length a))))
   (p: permission{allows_read p})
   (i:U32.t{U32.v i < U32.v (length a)})
+  (pre: Ghost.erased (Preorder.preorder t))
   : action
-    (pts_to_array a p iseq)
+    (pts_to_array_with_preorder a p iseq pre)
     (as:(array_ref t & array_ref t){(
       length (fst as) = i /\ length (snd as) = U32.sub (length a) i /\
       offset (fst as) = offset a /\ offset (snd as) = U32.add (offset a) i /\
@@ -1156,23 +1123,12 @@ let split_array_action
       address (fst as) = address a /\ address (snd as) = address a
     )})
     (fun (a1, a2) -> star
-      (pts_to_array a1 p (Seq.slice iseq 0 (U32.v i)))
-      (pts_to_array a2 p (Seq.slice iseq (U32.v i) (U32.v (length a))))
+      (pts_to_array_with_preorder a1 p (Seq.slice iseq 0 (U32.v i)) pre)
+      (pts_to_array_with_preorder a2 p (Seq.slice iseq (U32.v i) (U32.v (length a))) pre)
     )
   =
   pre_action_to_action
-    (pts_to_array a p iseq)
-    (as:(array_ref t & array_ref t){(
-      length (fst as) = i /\ length (snd as) = U32.sub (length a) i /\
-      offset (fst as) = offset a /\ offset (snd as) = U32.add (offset a) i /\
-      max_length (fst as) = max_length a /\ max_length (snd as) = max_length a /\
-      address (fst as) = address a /\ address (snd as) = address a
-    )})
-    (fun (a1, a2) -> star
-      (pts_to_array a1 p (Seq.slice iseq 0 (U32.v i)))
-      (pts_to_array a2 p (Seq.slice iseq (U32.v i) (U32.v (length a))))
-    )
-    (split_array_pre_action a iseq p i)
+    (split_array_pre_action a iseq p i pre)
     (fun frame h0 h1 addr -> ())
     (fun frame h0 h1 addr -> ())
     (fun frame h0 h1 -> ())
@@ -1198,20 +1154,8 @@ let split_array
     )
   =
   non_alloc_action_to_non_locking_m_action
-    (pts_to_array a p iseq)
-    (as:(array_ref t & array_ref t){(
-      length (fst as) = i /\ length (snd as) = U32.sub (length a) i /\
-      offset (fst as) = offset a /\ offset (snd as) = U32.add (offset a) i /\
-      max_length (fst as) = max_length a /\ max_length (snd as) = max_length a /\
-      address (fst as) = address a /\ address (snd as) = address a
-    )})
-    (fun (a1, a2) -> star
-      (pts_to_array a1 p (Seq.slice iseq 0 (U32.v i)))
-      (pts_to_array a2 p (Seq.slice iseq (U32.v i) (U32.v (length a))))
-    )
-    (split_array_action a iseq p i)
+    (split_array_action a iseq p i (trivial_preorder t))
     (fun h addr -> ())
-
 
 #push-options "--max_fuel 2 --initial_fuel 2 --max_ifuel 1 --initial_ifuel 1 --z3rlimit 30"
 let glue_array_pre_action
@@ -1224,13 +1168,14 @@ let glue_array_pre_action
   (iseq: Ghost.erased (Seq.lseq t (U32.v (length a))))
   (iseq': Ghost.erased (Seq.lseq t (U32.v (length a'))))
   (p: permission{allows_read p})
+  (pre: Ghost.erased (Preorder.preorder t))
   : pre_action
-    (star (pts_to_array a p iseq) (pts_to_array a' p iseq'))
+    (star (pts_to_array_with_preorder a p iseq pre) (pts_to_array_with_preorder a' p iseq' pre))
     (new_a:array_ref t{
       address new_a = address a /\ max_length new_a = max_length a /\
       offset new_a = offset a /\ length new_a = U32.add (length a) (length a')
     })
-    (fun new_a -> pts_to_array new_a p (Seq.Base.append iseq iseq'))
+    (fun new_a -> pts_to_array_with_preorder new_a p (Seq.Base.append iseq iseq') pre)
   = fun h ->
   let new_a : array_ref t = { a with array_length = U32.add a.array_length a'.array_length} in
   (| new_a, h |)
@@ -1247,22 +1192,17 @@ let glue_array_action
   (iseq: Ghost.erased (Seq.lseq t (U32.v (length a))))
   (iseq': Ghost.erased (Seq.lseq t (U32.v (length a'))))
   (p: permission{allows_read p})
+  (pre: Ghost.erased (Preorder.preorder t))
   : action
-    (star (pts_to_array a p iseq) (pts_to_array a' p iseq'))
+    (star (pts_to_array_with_preorder a p iseq pre) (pts_to_array_with_preorder a' p iseq' pre))
     (new_a:array_ref t{
       address new_a = address a /\ max_length new_a = max_length a /\
       offset new_a = offset a /\ length new_a = U32.add (length a) (length a')
     })
-    (fun new_a -> pts_to_array new_a p (Seq.Base.append iseq iseq'))
+    (fun new_a -> pts_to_array_with_preorder new_a p (Seq.Base.append iseq iseq') pre)
   =
   pre_action_to_action
-    (star (pts_to_array a p iseq) (pts_to_array a' p iseq'))
-    (new_a:array_ref t{
-      address new_a = address a /\ max_length new_a = max_length a /\
-      offset new_a = offset a /\ length new_a = U32.add (length a) (length a')
-    })
-    (fun new_a -> pts_to_array new_a p (Seq.Base.append iseq iseq'))
-    (glue_array_pre_action a a' iseq iseq' p)
+    (glue_array_pre_action a a' iseq iseq' p pre)
     (fun frame h0 h1 addr -> ())
     (fun frame h0 h1 addr -> ())
     (fun frame h0 h1 -> ())
@@ -1287,13 +1227,7 @@ let glue_array
     (fun new_a -> pts_to_array new_a p (Seq.Base.append iseq iseq'))
   =
   non_alloc_action_to_non_locking_m_action
-    (star (pts_to_array a p iseq) (pts_to_array a' p iseq'))
-    (new_a:array_ref t{
-      address new_a = address a /\ max_length new_a = max_length a /\
-      offset new_a = offset a /\ length new_a = U32.add (length a) (length a')
-    })
-    (fun new_a -> pts_to_array new_a p (Seq.Base.append iseq iseq'))
-    (glue_array_action a a' iseq iseq' p)
+    (glue_array_action a a' iseq iseq' p (trivial_preorder t))
     (fun h addr -> ())
 
 ///////////////////////////////////////////////////////////////////////////////
@@ -1308,9 +1242,6 @@ let rewrite_hprop_pre (p:hprop) (p':hprop{p `equiv` p'})
 let rewrite_hprop_action (p:hprop) (p':hprop{p `equiv` p'})
   : action p unit (fun _ -> p') =
   pre_action_to_action
-    p
-    (x:unit)
-    (fun _ -> p')
     (rewrite_hprop_pre p p')
     (fun frame h0 h1 addr -> ())
     (fun frame h0 h1 addr -> ())
@@ -1319,9 +1250,6 @@ let rewrite_hprop_action (p:hprop) (p':hprop{p `equiv` p'})
 
 let rewrite_hprop p p' =
   non_alloc_action_to_non_locking_m_action
-    p
-    (x:unit)
-    (fun _ -> p')
     (rewrite_hprop_action p p')
     (fun h0 addr -> ())
 
@@ -1329,35 +1257,62 @@ let rewrite_hprop p p' =
 // References
 ///////////////////////////////////////////////////////////////////////////////
 
-#push-options "--max_fuel 2 --initial_fuel 2"
-let sel_ref (#t: Type0) (r: reference t) (h: hheap (ref r)) : t =
-  Seq.index (as_seq r h) 0
+#push-options "--max_fuel 2 --initial_fuel 2 --max_ifuel 1 --initial_ifuel 1"
+let sel_ref
+  (#t: Type0)
+  (r: reference t)
+  (pre: Ghost.erased (Preorder.preorder t))
+  (m: hmem (ref r pre))
+  : t =
+  affine_star (ref r pre) (locks_invariant m) (heap_of_mem m);
+  assert(exists (p:permission{allows_read p}) (contents: Ghost.erased t).
+    interp (pts_to_ref r p contents pre) (heap_of_mem m)
+  );
+  let Array t' len' seq = select_addr (heap_of_mem m) r.array_addr in
+  let x =  select_index seq 0 in
+  x.value
 #pop-options
 
-#push-options "--max_fuel 2 --initial_fuel 2"
+#push-options "--max_fuel 2 --initial_fuel 2 --initial_fuel 1 --max_fuel 1 --z3rlimit 50"
 let sel_ref_lemma
   (t: Type0)
   (p: permission{allows_read p})
   (r: reference t)
-  (m: hheap (ref_perm r p))
-  : Lemma (interp (ref r) m /\ interp (pts_to_ref r p (sel_ref r m)) m)
+  (pre: Preorder.preorder t)
+  (m: hmem (ref_perm r p pre))
+  : Lemma (
+    interp (ref r pre `star` locks_invariant m) (heap_of_mem m) /\
+    interp (pts_to_ref r p (sel_ref r pre m) pre `star` locks_invariant m) (heap_of_mem m)
+  )
   =
-  ()
+  affine_star (ref_perm r p pre) (locks_invariant m) (heap_of_mem m);
+  assert(exists (contents: Ghost.erased t).
+    interp (pts_to_ref r p contents pre) (heap_of_mem m)
+  );
+  admit()
 #pop-options
 
 let get_ref_pre_action
   (#t: Type0)
   (r: reference t)
   (p: permission{allows_read p})
+  (pre: Ghost.erased (Preorder.preorder t))
   : pre_action
-    (ref_perm r p)
+    (ref_perm r p pre)
     (x:t)
-    (fun x -> pts_to_ref r p x)
+    (fun x -> pts_to_ref r p x pre)
   = fun h ->
-  let contents = sel_ref r h in
-  sel_ref_lemma t p r h;
-  let (| x, h' |) = index_array_pre_action r (Seq.create 1 contents) 0ul p h in
-  (| x, h' |)
+  let contents = sel_ref r pre h in
+  sel_ref_lemma t p r pre h;
+  let  x = match h r.array_addr with
+    | Some (Array t' len seq) ->
+      assert(contains_index seq 0);
+      match Seq.index seq 0 with
+      | None -> ()
+      | Some x -> x.value
+    | _ -> ()
+  in
+  (| x, h |)
 
 
 #push-options "--z3rlimit 50 --max_fuel 2 --initial_fuel 2 --initial_ifuel 1 --max_ifuel 1"
@@ -1365,16 +1320,14 @@ let get_ref_action
   (#t: Type0)
   (r: reference t)
   (p: permission{allows_read p})
+  (pre: Ghost.erased (Preorder.preorder t))
   : action
-    (ref_perm r p)
+    (ref_perm r p pre)
     (x:t)
-    (fun x -> pts_to_ref r p x)
+    (fun x -> pts_to_ref r p x pre)
   =
   pre_action_to_action
-    (ref_perm r p)
-    (x:t)
-    (fun x -> pts_to_ref r p x)
-    (get_ref_pre_action r p)
+    (get_ref_pre_action r p pre)
     (fun frame h0 h1 addr -> ())
     (fun frame h0 h1 addr -> ())
     (fun frame h0 h1  -> ())
@@ -1384,113 +1337,115 @@ let get_ref
   (#t: Type0)
   (r: reference t)
   (p: permission{allows_read p})
+  (pre: Ghost.erased (Preorder.preorder t))
   : m_action
-    (ref_perm r p)
+    (ref_perm r p pre)
     (x:t)
-    (fun x -> pts_to_ref r p x)
+    (fun x -> pts_to_ref r p x pre)
   =
   non_alloc_action_to_non_locking_m_action
-    (ref_perm r p)
-    (x:t)
-    (fun x -> pts_to_ref r p x)
-    (get_ref_action r p)
+    (get_ref_action r p pre)
     (fun h0 addr -> ())
 
+#push-options "--max_fuel 2 --initial_fuel 2"
 let set_ref_pre_action
   (#t: Type0)
   (r: reference t)
+  (old_v: Ghost.erased t)
   (v: t)
+  (pre: (Ghost.erased (Preorder.preorder t)){(Ghost.reveal pre) old_v v})
   : pre_action
-    (ref_perm r full_permission)
+    (pts_to_ref r full_permission old_v pre)
     unit
-    (fun _ -> pts_to_ref r full_permission v)
+    (fun _ -> pts_to_ref r full_permission v pre)
   = fun h ->
-  let contents = sel_ref r h in
-  sel_ref_lemma t full_permission r h;
+  let contents = sel_ref r pre h in
+  sel_ref_lemma t full_permission r pre h;
   assert(Seq.upd (Seq.create 1 contents) 0 v `Seq.equal` Seq.create 1 v);
-  upd_array_pre_action r (Seq.create 1 contents) 0ul v h
+  upd_array_pre_action r (Seq.create 1 contents) 0ul v pre h
+#pop-options
 
+#push-options "--max_fuel 2 --initial_fuel 2"
 let set_ref_action
   (#t: Type0)
   (r: reference t)
+  (old_v: Ghost.erased t)
   (v: t)
+  (pre: (Ghost.erased (Preorder.preorder t)){(Ghost.reveal pre) old_v v})
   : action
-    (ref_perm r full_permission)
+    (pts_to_ref r full_permission old_v pre)
     unit
-    (fun _ -> pts_to_ref r full_permission v)
+    (fun _ -> pts_to_ref r full_permission v pre)
   =
   pre_action_to_action
-    (ref_perm r full_permission)
-    unit
-    (fun _ -> pts_to_ref r full_permission v)
-    (set_ref_pre_action r v)
+    (set_ref_pre_action r old_v v pre)
      (fun frame h0 h1 addr -> (* Disjointness preservation *)
-     let iseq = Seq.create 1 (sel_ref r h0) in
-     sel_ref_lemma t full_permission r h0;
-      upd_array_heap_frame_disjointness_preservation r iseq 0ul v (join h0 h1) h0 h1 frame
+      let iseq = Seq.create 1 (sel_ref r pre h0) in
+      sel_ref_lemma t full_permission r pre h0;
+      upd_array_heap_frame_disjointness_preservation r iseq 0ul v pre (join h0 h1) h0 h1 frame
     )
     (fun frame h0 h1 addr -> (* Does not depend on framing *)
-      let iseq = Seq.create 1 (sel_ref r h0) in
-      sel_ref_lemma t full_permission r h0;
-      upd_array_action_memory_split_independence r iseq 0ul v (join h0 h1) h0 h1 frame
+      let iseq = Seq.create 1 (sel_ref r pre h0) in
+      sel_ref_lemma t full_permission r pre h0;
+      upd_array_action_memory_split_independence r iseq 0ul v pre (join h0 h1) h0 h1 frame
     )
     (fun frame h0 h1  -> (* Return and post *)
-      let iseq = Seq.create 1 (sel_ref r h0) in
-      sel_ref_lemma t full_permission r h0;
-      let (| x0, h |) = set_ref_pre_action r v h0 in
-      let (| x1, h' |) = set_ref_pre_action r v (join h0 h1) in
+      let iseq = Seq.create 1 (sel_ref r pre h0) in
+      sel_ref_lemma t full_permission r pre h0;
+      let (| x0, h |) = set_ref_pre_action r old_v v pre h0 in
+      let (| x1, h' |) = set_ref_pre_action r old_v v pre (join h0 h1) in
       assert (x0 == x1)
     )
+#pop-options
 
 let set_ref
   (#t: Type0)
   (r: reference t)
+  (old_v: Ghost.erased t)
   (v: t)
+  (pre: (Ghost.erased (Preorder.preorder t)){(Ghost.reveal pre) old_v v})
   : m_action
-    (ref_perm r full_permission)
+    (pts_to_ref r full_permission old_v pre)
     unit
-    (fun _ -> pts_to_ref r full_permission v)
+    (fun _ -> pts_to_ref r full_permission v pre)
   =
   non_alloc_action_to_non_locking_m_action
-    (ref_perm r full_permission)
-    unit
-    (fun _ -> pts_to_ref r full_permission v)
-    (set_ref_action r v)
+    (set_ref_action r old_v v pre)
     (fun h0 addr -> ())
 
 let alloc_ref
   (#t: Type0)
   (v: t)
+  (pre: Ghost.erased (Preorder.preorder t))
   : m_action
     emp
     (reference t)
-    (fun r -> pts_to_ref r full_permission v)
+    (fun r -> pts_to_ref r full_permission v pre)
   =
-  alloc_array 1ul v
+  alloc_array_is_m_frame_and_preorder_preserving 1ul v pre;
+  alloc_array_pre_m_action 1ul v pre
 
 let free_ref_pre_action
   (#t: Type0)
   (r: reference t)
+  (pre: Ghost.erased (Preorder.preorder t))
   : pre_action
-    (ref_perm r full_permission)
+    (ref_perm r full_permission pre)
     unit
     (fun _ -> emp)
-  = fun h ->
-    free_array_pre_action r h
+  = fun h -> (| (), h |)
 
 let free_ref_action
   (#t: Type0)
   (r: reference t)
+  (pre: Ghost.erased (Preorder.preorder t))
   : pre_action
-    (ref_perm r full_permission)
+    (ref_perm r full_permission pre)
     unit
     (fun _ -> emp)
   =
   pre_action_to_action
-    (ref_perm r full_permission)
-    unit
-    (fun _ -> emp)
-    (free_ref_pre_action r)
+    (free_ref_pre_action r pre)
     (fun frame h0 h1 addr -> ())
     (fun frame h0 h1 addr -> ())
     (fun frame h0 h1 -> ())
@@ -1500,16 +1455,14 @@ let free_ref_action
 let free_ref
   (#t: Type0)
   (r: reference t)
+  (pre: Ghost.erased (Preorder.preorder t))
   : m_action
-    (ref_perm r full_permission)
+    (ref_perm r full_permission pre)
     unit
     (fun _ -> emp)
   =
   non_alloc_action_to_non_locking_m_action
-    (ref_perm r full_permission)
-    unit
-    (fun _ -> emp)
-    (free_ref_action r)
+    (free_ref_action r pre)
     (fun h0 addr -> ())
 #pop-options
 
@@ -1518,15 +1471,18 @@ let share_ref
   (r: reference t)
   (p: permission{allows_read p})
   (contents: Ghost.erased t)
+  (pre: Ghost.erased (Preorder.preorder t))
   : m_action
-    (pts_to_ref r p contents)
+    (pts_to_ref r p contents pre)
     (r':reference t{ref_address r' = ref_address r})
     (fun r' ->
-      pts_to_ref r (half_permission p) contents `star`
-      pts_to_ref r' (half_permission p) contents
+      pts_to_ref r (half_permission p) contents pre `star`
+      pts_to_ref r' (half_permission p) contents pre
     )
   =
-  share_array r (Seq.create 1 (Ghost.reveal contents)) p
+   non_alloc_action_to_non_locking_m_action
+      (share_array_action r (Seq.create 1 (Ghost.reveal contents)) p pre)
+      (fun h addr -> ())
 
 let gather_ref
   (#t: Type0)
@@ -1535,13 +1491,16 @@ let gather_ref
   (p: permission{allows_read p})
   (p': permission{allows_read p' /\ summable_permissions p p'})
   (contents: Ghost.erased t)
+  (pre: Ghost.erased (Preorder.preorder t))
   : m_action
-    (pts_to_ref r p contents `star`
-      pts_to_ref r' p' contents)
+    (pts_to_ref r p contents pre `star`
+      pts_to_ref r' p' contents pre)
     unit
-    (fun _ -> pts_to_ref r (sum_permissions p p') contents)
+    (fun _ -> pts_to_ref r (sum_permissions p p') contents pre)
   =
-  gather_array r r' (Seq.create 1 (Ghost.reveal contents)) p p'
+  non_alloc_action_to_non_locking_m_action
+    (gather_array_action r r' (Seq.create 1 (Ghost.reveal contents)) p p' pre)
+    (fun h addr -> ())
 
 
 ////////////////////////////////////////////////////////////////////////////////
