pulse/ulib/experimental/Steel.Memory.fsti
@@ -114,7 +114,7 @@ val pts_to_array_with_preorder
   (contents:Ghost.erased (Seq.lseq t (U32.v (length a))))
   (preorder: Ghost.erased (Preorder.preorder t))
   : hprop
-val pts_to_ref_with_preorder
+val pts_to_ref
   (#t: Type0)
   (r: reference t)
   (p:permission{allows_read p})
@@ -173,19 +173,18 @@ val pts_to_array_injective
 // pts_to_ref and abbreviations
 ////////////////////////////////////////////////////////////////////////////////
 
-let pts_to_ref
+let ref_perm
   (#t: Type0)
   (r: reference t)
   (p:permission{allows_read p})
-  (contents: Ghost.erased t)
+  (pre: Ghost.erased (Preorder.preorder t))
   : hprop =
-  pts_to_ref_with_preorder r p contents (Ghost.hide (trivial_preorder t))
+  h_exists (fun (contents: Ghost.erased t) ->
+    pts_to_ref r p contents pre
+  )
 
-let ref_perm (#t: Type0) (r: reference t) (p:permission{allows_read p}) : hprop
-  = h_exists (pts_to_ref r p)
-
-let ref (#t: Type0) (r: reference t) : hprop
-  = h_exists (fun (p:permission{allows_read p}) -> ref_perm r p)
+let ref (#t: Type0) (r: reference t) (pre: Ghost.erased (Preorder.preorder t)) : hprop
+  = h_exists (fun (p:permission{allows_read p}) -> ref_perm r p pre)
 
 val pts_to_ref_injective
   (#t: _)
@@ -196,8 +195,8 @@ val pts_to_ref_injective
   (m: heap)
   : Lemma
     (requires (
-      interp (pts_to_ref_with_preorder a p c0 pre) m /\
-      interp (pts_to_ref_with_preorder a p c1 pre) m))
+      interp (pts_to_ref a p c0 pre) m /\
+      interp (pts_to_ref a p c1 pre) m))
     (ensures (c0 == c1))
 
 ////////////////////////////////////////////////////////////////////////////////
