pulse/ulib/experimental/Steel.Actions.fsti
@@ -189,49 +189,63 @@ val glue_array
 val rewrite_hprop (p:hprop) (p':hprop{p `equiv` p'}) : m_action p unit (fun _ -> p')
 
 ///////////////////////////////////////////////////////////////////////////////
-// References
+// References with preorders
 ///////////////////////////////////////////////////////////////////////////////
 
-val sel_ref (#t: Type0) (r: reference t) (h: hheap (ref r)) : t
+val sel_ref
+  (#t: Type0)
+  (r: reference t)
+  (pre: Ghost.erased (Preorder.preorder t))
+  (h: hmem (ref r pre))
+  : Tot t
 
 val sel_ref_lemma
   (t: Type0)
   (p: permission{allows_read p})
   (r: reference t)
-  (m: hheap (ref_perm r p))
-  : Lemma (interp (ref r) m /\ interp (pts_to_ref r p (sel_ref r m)) m)
+  (pre: Preorder.preorder t)
+  (m: hmem (ref_perm r p pre))
+  : Lemma (
+    interp (ref r pre `star` locks_invariant m) (heap_of_mem m) /\
+    interp (pts_to_ref r p (sel_ref r pre m) pre `star` locks_invariant m) (heap_of_mem m)
+  )
 
 val get_ref
   (#t: Type0)
   (r: reference t)
   (p: permission{allows_read p})
+  (pre: Ghost.erased (Preorder.preorder t))
   : m_action
-    (ref_perm r p)
+    (ref_perm r p pre)
     (x:t)
-    (fun x -> pts_to_ref r p x)
+    (fun x -> pts_to_ref r p x pre)
 
 val set_ref
   (#t: Type0)
   (r: reference t)
+  (old_v: Ghost.erased t)
   (v: t)
+  (pre: (Ghost.erased (Preorder.preorder t)){(Ghost.reveal pre) old_v v})
   : m_action
-    (ref_perm r full_permission)
+    (pts_to_ref r full_permission old_v pre)
     unit
-    (fun _ -> pts_to_ref r full_permission v)
+    (fun _ -> pts_to_ref r full_permission v pre)
 
 val alloc_ref
   (#t: Type0)
   (v: t)
+  (pre: Ghost.erased (Preorder.preorder t))
   : m_action
     emp
     (reference t)
-    (fun r -> pts_to_ref r full_permission v)
+    (fun r -> pts_to_ref r full_permission v pre)
 
 val free_ref
   (#t: Type0)
   (r: reference t)
+  (pre: Ghost.erased (Preorder.preorder t))
   : m_action
-    (ref_perm r full_permission)
+    (ref_perm r full_permission pre)
     unit
     (fun _ -> emp)
 
@@ -240,12 +254,13 @@ val share_ref
   (r: reference t)
   (p: permission{allows_read p})
   (contents: Ghost.erased t)
+  (pre: Ghost.erased (Preorder.preorder t))
   : m_action
-    (pts_to_ref r p contents)
+    (pts_to_ref r p contents pre)
     (r':reference t{ref_address r' = ref_address r})
     (fun r' ->
-      pts_to_ref r (half_permission p) contents `star`
-      pts_to_ref r' (half_permission p) contents
+      pts_to_ref r (half_permission p) contents pre `star`
+      pts_to_ref r' (half_permission p) contents pre
     )
 
 val gather_ref
@@ -255,11 +270,12 @@ val gather_ref
   (p: permission{allows_read p})
   (p': permission{allows_read p' /\ summable_permissions p p'})
   (contents: Ghost.erased t)
+  (pre: Ghost.erased (Preorder.preorder t))
   : m_action
-    (pts_to_ref r p contents `star`
-      pts_to_ref r' p' contents)
+    (pts_to_ref r p contents pre `star`
+      pts_to_ref r' p' contents pre)
     unit
-    (fun _ -> pts_to_ref r (sum_permissions p p') contents)
+    (fun _ -> pts_to_ref r (sum_permissions p p') contents pre)
 
 ///////////////////////////////////////////////////////////////////////////////
 // Locks
